thread log map

steel/Zeta.Steel.ThreadLogMap.fst
@@ -5,8 +5,8 @@ open Zeta.Steel.FormatsManual
 open Zeta.Steel.ApplicationTypes
 open Zeta.Steel.ApplicationTypes
 open Steel.ST.Util
-module FAP = Zeta.Steel.FractionalAnchoredPreorder
-module PM = Zeta.Steel.PCMMap
+module FAP = Steel.FractionalAnchoredPreorder
+module PM = Steel.PCMMap
 module M = Zeta.Steel.ThreadStateModel
 
 let log = Seq.seq log_entry_base
@@ -21,20 +21,19 @@ let log_grows :Preorder.preorder log
 let committed_log_entries_split (l0 l1 l2: log)
   : Lemma
     (requires
-      M.committed_log_entries l0 == M.committed_log_entries l2 /\
+      l0 == M.committed_log_entries l2 /\
       log_grows l0 l1 /\
       log_grows l1 l2)
     (ensures
-            M.committed_log_entries l0 == M.committed_log_entries l1)
+      l0 == M.committed_log_entries l1)
   = admit()
 
 
 let anchor : log -> log -> prop
   = fun l0 l1 ->
       log_grows l0 l1 /\
-      M.committed_log_entries l0 == M.committed_log_entries l1
+      l0 == M.committed_log_entries l1
 
-let anchor_refl : squash (forall l. anchor l l) = ()
 let anchor_pre : squash (forall l0 l1. anchor l0 l1 ==> log_grows l0 l1) = ()
 let anchor_split : squash (forall x z. x `anchor` z  ==> (forall y. log_grows x y /\ log_grows y z ==> x `anchor` y)) =
   introduce forall x. _
@@ -56,17 +55,20 @@ let avalue_of (m:PM.map tid aval) (tid:tid { has_key m tid }) =
   (FAP.Owns?._0 (Map.sel m tid))
 let get (m:PM.map tid aval) (tid:tid { has_key m tid }) =
   Steel.Preorder.curval (FAP.avalue_val (avalue_of m tid))
-let put (m:PM.map tid aval) (tid:tid { has_key m tid }) (l:log {get m tid `log_grows` l}) =
-  Map.upd m tid (FAP.Owns (FAP.avalue_update_value (FAP.Owns?._0 (Map.sel m tid)) l))
+let put (m:PM.map tid aval)
+        (tid:tid { has_key m tid })
+        (l:log {get m tid `log_grows` l /\ anchors l l})
+  = Map.upd m tid (FAP.Owns (FAP.avalue_update_value (FAP.Owns?._0 (Map.sel m tid)) l))
 
 let update_value (l:log)
                  (m:PM.map tid aval)
                  (tid:tid {
                    owns_key m tid /\ //if you have full ownership of key
-                   get m tid `log_grows` l //you can update it wrt the preorder only
+                   get m tid `log_grows` l /\ //you can update it wrt the preorder only
+                   anchors l l
                  })
   : PCM.frame_preserving_upd pcm m (put m tid l)
-  = PM.lift_fp_upd _ _ (FAP.update_value (FAP.Owns?._0 (Map.sel m tid)) l) m tid
+  = PM.lift_frame_preserving_upd _ _ (FAP.update_value (FAP.Owns?._0 (Map.sel m tid)) l) m tid
 
 let owns_anchored_key (m:PM.map tid aval) (tid:tid) =
   has_key m tid /\
@@ -88,4 +90,294 @@ let update_anchored_value (l:log)
                             l `FAP.compat_with_any_anchor_of` (avalue_of m tid) //and respect any anchor of the current value
                           })
   : PCM.frame_preserving_upd pcm m (put_anchored m tid l)
-  = PM.lift_fp_upd _ _ (FAP.update_anchored_value (FAP.Owns?._0 (Map.sel m tid)) l) m tid
+  = PM.lift_frame_preserving_upd _ _ (FAP.update_anchored_value (FAP.Owns?._0 (Map.sel m tid)) l) m tid
+
+// // ////////////////////////////////////////////////////////////////////////////////
+
+// // let tmap (k:eqtype) (v:Type0) (c:preorder v) = Map.t k (hist c)
+module G = Steel.ST.GhostPCMReference
+
+let t = G.ref _ pcm
+
+let no_ownership (m:PM.map tid aval) (tid:tid) =
+  not (has_key m tid) \/
+  (let (p, _) = FAP.Owns?._0 (Map.sel m tid) in
+   None? (fst p) /\
+   None? (snd p))
+
+let has_anchor (m:PM.map tid aval) (tid:tid) =
+  has_key m tid /\
+  (let p, _ = FAP.Owns?._0 (Map.sel m tid) in
+   Some? (snd p))
+
+let perm_of (m:PM.map tid aval) (tid:tid { has_key m tid }) =
+  let p, _ = FAP.Owns?._0 (Map.sel m tid) in
+  fst p
+
+let anchor_of (m:PM.map tid aval) (t:tid{ has_anchor m t }) =
+  let p, _ = FAP.Owns?._0 (Map.sel m t) in
+  Some?.v (snd p)
+
+let owns_anchor_only (m:PM.map tid aval) (tid:tid) =
+  has_anchor m tid /\
+  None? (perm_of m tid)
+
+let global_anchor_pred (x:t) (m:PM.map tid (option log)) (m':PM.map tid aval)
+  : prop
+  = forall tid.
+      match Map.sel m tid with
+      | None ->
+        not (has_key m' tid)
+      | Some l ->
+        owns_anchor_only m' tid /\
+        get m' tid == l /\
+        anchor_of m' tid == l
+
+assume
+val global_anchor (x:t) ([@@@smt_fallback] m:PM.map tid (option log))
+  : vprop
+  // = exists_ (fun m' ->
+  //     G.pts_to x m' `star`
+  //     pure (global_anchor_pred x m m'))
+
+let intro_global_anchor (#o:_) (x:t) (m:PM.map tid (option log)) (m':PM.map tid aval)
+  : STGhost unit o
+       (G.pts_to x m')
+       (fun _ -> global_anchor x m)
+       (requires global_anchor_pred x m m')
+       (ensures fun _ -> True)
+  = admit_()
+    // intro_pure (global_anchor_pred x m m');
+    // intro_exists m' (fun m' ->
+    //   G.pts_to x m' `star`
+    //   pure (global_anchor_pred x m m'))
+
+let global_snapshot (x:t) ([@@@smt_fallback] m: PM.map tid log)
+  : vprop
+  = exists_ (fun m' ->
+      G.pts_to x m' `star`
+      pure (forall tid. has_key m' tid /\
+                   get m' tid == Map.sel m tid /\
+                   no_ownership m' tid))
+
+let tid_pts_to (x:t)
+               (tid:tid)
+               ([@@@smt_fallback] frac:perm)
+               ([@@@smt_fallback]  l:log) =
+  exists_ (fun m ->
+    G.pts_to x m `star`
+    pure (forall t. if t=tid
+               then (
+                 has_key m t /\
+                 perm_of m tid == Some frac /\
+                 ~ (has_anchor m tid) /\
+                 get m t == l
+               )
+               else (
+                 not (has_key m t)
+               )))
+
+let tids_pts_to_pred (x:t) (frac:perm) (m:PM.map tid (option log)) (m': PM.map tid aval)
+  : prop
+  = forall tid.
+      match Map.sel m tid with
+      | None -> not (has_key m' tid)
+      | Some l ->
+        has_key m' tid /\
+        perm_of m' tid == Some frac /\
+        get m' tid == l /\
+        ~ (has_anchor m' tid)
+
+assume
+val tids_pts_to (x:t) ([@@@smt_fallback] frac:perm) ([@@@smt_fallback] m:PM.map tid (option log))
+  : vprop
+  // exists_ (fun m' ->
+  //   G.pts_to x m' `star`
+  //   pure (tids_pts_to_pred x frac m m'))
+
+let intro_tids_pts_to (#o:_) (x:t) (frac:perm) (m:PM.map tid (option log)) (m':PM.map tid aval)
+  : STGhost unit o
+       (G.pts_to x m')
+       (fun _ -> tids_pts_to x frac m)
+       (requires tids_pts_to_pred x frac m m')
+       (ensures fun _ -> True)
+  = intro_pure (tids_pts_to_pred x frac m m');
+    intro_exists m' (fun m' ->
+      G.pts_to x m' `star`
+      pure (tids_pts_to_pred x frac m m'));
+    admit_()
+
+let alloc0 (#o:_) (_:unit)
+  : STGhostT t o
+             emp
+             (fun t -> G.pts_to t (Map.const (FAP.Owns (FAP.initial_value Seq.empty))))
+  = G.alloc (Map.const (FAP.Owns (FAP.initial_value Seq.empty)))
+
+let map_map (m:PM.map tid aval)
+            (f:(tid:tid -> a:FAP.avalue anchors{ Map.sel m tid == FAP.Owns a } -> FAP.avalue anchors))
+  : PM.map tid aval
+  = Map.map_literal (fun tid ->
+       match Map.sel m tid with
+       | FAP.Owns m -> FAP.Owns (f tid m)
+       | FAP.Nothing -> FAP.Nothing)
+
+let split_anchor (m:PM.map tid aval)
+  : Lemma
+    (requires
+      forall (k:_{has_key m k}).{:pattern (Map.sel m k)}
+        anchors (get m k) (get m k) /\
+        owns_key m k)
+    (ensures
+      PM.composable_maps fap
+        (map_map m (fun _ a -> fst (FAP.anchored_snapshot a)))
+        (map_map m (fun _ a -> snd (FAP.anchored_snapshot a))) /\
+      m `Map.equal` PM.compose_maps fap
+           (map_map m (fun _ a -> fst (FAP.anchored_snapshot a)))
+           (map_map m (fun _ a -> snd (FAP.anchored_snapshot a)))
+      )
+  = ()
+
+let alloc (#o:_) (_:unit)
+  : STGhostT t o
+             emp
+             (fun t -> tids_pts_to t full_perm (Map.const (Some Seq.empty)) `star`
+                    global_anchor t (Map.const (Some Seq.empty)))
+  = let m = (Map.const (FAP.Owns (FAP.initial_value Seq.empty))) in
+    let x = alloc0 () in
+    rewrite (G.pts_to x _)
+            (G.pts_to x m);
+    split_anchor m;
+    let m0 = map_map m (fun _ a -> fst (FAP.anchored_snapshot a)) in
+    let m1 = map_map m (fun _ a -> snd (FAP.anchored_snapshot a)) in
+    G.share x m m0 m1;
+    assert_ (G.pts_to x m0 `star` G.pts_to x m1);
+    let mm0 : PM.map tid (option log) = Map.const (Some Seq.empty) in
+    intro_tids_pts_to x full_perm mm0 m0;
+    intro_global_anchor x mm0 m1;
+    x
+
+
+let share_tid_pts_to (#o:_) (#f:perm) (x:t) (m:PM.map tid (option log))
+  : STGhostT unit o
+    (tids_pts_to x f m)
+    (fun _ -> tids_pts_to x (half_perm f) m `star` tids_pts_to x (half_perm f) m)
+  = admit_()
+
+let take_tid (#o:_) (#f:perm) (x:t) (m:PM.map tid (option log)) (tid:tid { Some? (Map.sel m tid) })
+  : STGhostT unit o
+    (tids_pts_to x f m)
+    (fun _ -> tid_pts_to x tid f (Some?.v (Map.sel m tid)) `star`
+           tids_pts_to x (half_perm f) (Map.upd m tid None))
+  = admit_()
+
+
+
+
+
+//                perm_ok (Map.sel m t)))
+
+// val global_snapshot (x:t) (m:map tid log)
+//   : vprop
+//   = G.pts_to x m `star`
+//   exists_ (fun (km:kmap k v c) ->
+//         pure (snapshot km == m) `star`
+//         k_of t (Owns (ksnapshot km)))
+
+// // // val k_of (#k:eqtype) (#v:Type0) (#c:preorder v)
+// // //          (t:t k v c)
+// // //          (knowledge: knowledge k v c)
+// // //   : vprop
+
+// // // val share  (#o:_)
+// // //            (#k:eqtype) (#v:Type0) (#c:preorder v)
+// // //            (#m0 :kmap k v c)
+// // //            (#m1: kmap k v c { kmap_composable m0 m1 })
+// // //            (t:t k v c)
+// // //   : STGhostT unit o
+// // //     (k_of t (Owns (compose_kmaps m0 m1)))
+// // //     (fun _ -> k_of t (Owns m0) `star` k_of t (Owns m1))
+
+// // // val gather (#o:_)
+// // //            (#k:eqtype) (#v:Type0) (#c:preorder v)
+// // //            (#m0 #m1: kmap k v c)
+// // //            (t:t k v c)
+// // //   : STGhostT (_:unit { kmap_composable m0 m1 }) o
+// // //     (k_of t (Owns m0) `star` k_of t (Owns m1))
+// // //     (fun _ -> k_of t (Owns (compose_kmaps m0 m1)))
+
+
+// // // val take_snapshot (#o:_)
+// // //                   (#k:eqtype) (#v:Type0) (#c:preorder v)
+// // //                   (#m: kmap k v c)
+// // //                   (t:t k v c)
+// // //   : STGhostT unit o
+// // //     (k_of t (Owns m))
+// // //     (fun _ -> k_of t (Owns m) `star` global_snapshot t (snapshot m))
+
+// // // val owns_key (#k:eqtype) (#v:Type0) (#c:preorder v)
+// // //              (t:t k v c)
+// // //              (key:k)
+// // //              ([@@@smt_fallback]perm:perm)
+// // //              ([@@@smt_fallback]value:v)
+// // //  : vprop
+// // //   // = exists_ (fun (m:kmap k v c) ->
+// // //   //      pure ((forall key'. (key<>key' ==> fst (Map.sel m key') == None)) /\
+// // //   //            (match Map.sel m key with
+// // //   //             | None, _ -> False
+// // //   //             | Some p, h ->
+// // //   //               perm == p /\
+// // //   //               curval h == value)) `star`
+// // //   //      k_of t (Owns m))
+
+// // // val snapshot_of_key (#k:eqtype) (#v:Type0) (#c:preorder v)
+// // //                     (t:t k v c)
+// // //                     (key:k)
+// // //                     ([@@@smt_fallback]value:v)
+// // //  : vprop
+// // //   // = exists_ (fun (m:kmap k v c) ->
+// // //   //      pure ((forall key'. fst (Map.sel m key') == None) /\
+// // //   //            (match Map.sel m key with
+// // //   //             | Some _, _ -> False
+// // //   //             | None, h -> curval h == value)) `star`
+// // //   //      k_of t (Owns m))
+
+// // // val local_snapshot (#o:_)
+// // //                    (#k:eqtype) (#v:Type0) (#c:preorder v)
+// // //                    (#key:k) (#frac:_) (#value:v)
+// // //                    (t:t k v c)
+// // //   : STGhostT unit o
+// // //     (owns_key t key frac value)
+// // //     (fun _ -> owns_key t key frac value `star` snapshot_of_key t key value)
+
+// // // val dup_snapshot (#o:_)
+// // //                  (#k:eqtype) (#v:Type0) (#c:preorder v)
+// // //                  (#key:k) (#value:v)
+// // //                  (t:t k v c)
+// // //   : STGhostT unit o
+// // //     (snapshot_of_key t key value)
+// // //     (fun _ -> snapshot_of_key t key value `star` snapshot_of_key t key value)
+
+// // // val update (#o:_)
+// // //            (#k:eqtype) (#v:Type0) (#c:preorder v)
+// // //            (#key:k) (#value:v)
+// // //            (t:t k v c)
+// // //            (value':v {c value value'})
+// // //   : STGhostT unit o
+// // //     (owns_key t key full_perm value)
+// // //     (fun _ -> owns_key t key full_perm value')
+
+// // // val update_global_snapshot (#o:_)
+// // //                            (#k:eqtype) (#v:Type0) (#c:preorder v)
+// // //                            (#key:k) (#frac:_) (#value:v)
+// // //                            (t:t k v c)
+// // //                            (m:Map.t k v)
+// // //   : STGhostT unit o
+// // //     (owns_key t key frac value `star` global_snapshot t m)
+// // //     (fun _ -> owns_key t key frac value `star` global_snapshot t (Map.upd m key value))
+
+
+// // // val dup_global_snapshot (#o:_) (#k:eqtype) (#v:Type0) (#c:preorder v) (#m: Map.t k v)
+// // //                         (t:t k v c)
+// // //   : STGhostT unit o
+// // //     (global_snapshot t m)
+// // //     (fun _ -> global_snapshot t m `star` global_snapshot t m)
